thys/Flow_Networks/Lib/Fofu_Impl_Base.thy
@@ -3,46 +3,8 @@ imports
   "../../Refine_Imperative_HOL/IICF/IICF"
   "../../Refine_Imperative_HOL/Sepref_ICF_Bindings"
   "~~/src/HOL/Library/Rewrite"
-  Refine_Monadic_Syntax_Sugar
 begin
   hide_type (open) List_Seg.node
 
   interpretation Refine_Monadic_Syntax .
-
-
-      
-(* TODO: Move, patch Imperative/HOL! 
-  This patch makes Imperative/HOL array translation also work for index types other than IntInf.
-  Note that the toInt-operations are required to raise an Overflow exception on overflow, such that
-  creating an array of too big size is safe, and also indexing an array out of bounds will be 
-  correctly caught.
-*)
-code_printing constant Array.new' \<rightharpoonup> (SML) "(fn/ ()/ =>/ Array.array/ (IntInf.toInt _,/ (_)))"
-code_printing constant Array.make' \<rightharpoonup> (SML) "(fn/ ()/ =>/ Array.tabulate/ (IntInf.toInt _,/ _ o IntInf.fromInt))"
-code_printing constant Array.len' \<rightharpoonup> (SML) "(fn/ ()/ =>/ IntInf.fromInt (Array.length/ _))"
-code_printing constant Array.nth' \<rightharpoonup> (SML) "(fn/ ()/ =>/ Array.sub/ ((_),/ IntInf.toInt _))"
-code_printing constant Array.upd' \<rightharpoonup> (SML) "(fn/ ()/ =>/ Array.update/ ((_),/ IntInf.toInt _,/ (_)))"
-  
-  
-(*
-  TODO: Patch that belongs to array_blit.thy. 
-  Already in Lammich's local AFP copy!
-*)  
-code_printing code_module "array_blit" \<rightharpoonup> (SML)
-  {*
-  (* Locally patched version  *)
-  fun array_blit src si dst di len = (
-    src=dst andalso raise Fail ("array_blit: Same arrays");
-    ArraySlice.copy {
-      di = IntInf.toInt di,
-      src = ArraySlice.slice (src,IntInf.toInt si,SOME (IntInf.toInt len)),
-      dst = dst})
-
-  fun array_nth_oo v a i () = Array.sub(a,IntInf.toInt i) handle Subscript => v | Overflow => v
-  fun array_upd_oo f i x a () = 
-    (Array.update(a,IntInf.toInt i,x); a) handle Subscript => f () | Overflow => f ()
-
-  *}
-  
-  
 end
