thys/Flow_Networks/Lib/Refine_Add_Fofu.thy
@@ -1,8 +1,6 @@
 theory Refine_Add_Fofu
 imports 
   Fofu_Impl_Base 
-  Refine_Monadic_Syntax_Sugar
-  "DRAT_Misc"
   "../../DFS_Framework/Misc/DFS_Framework_Refine_Aux"
 begin
 
@@ -57,143 +55,8 @@ lemma vcg_rem_frame: "m\<le>m' \<Longrightarrow> VCG_FRAME m \<le> m'" unfolding
       
       
 
-  (* TODO: Integrate into Refinement Framework! *)
 
-  lemma LFO_pre_refine: (* TODO: Move and generalize! *)
-    assumes "(li,l)\<in>\<langle>A\<rangle>list_set_rel"
-    assumes "(ci,c)\<in>R \<rightarrow> bool_rel"
-    assumes "(fi,f)\<in>A\<rightarrow>R\<rightarrow>\<langle>R\<rangle>nres_rel"
-    assumes "(s0i,s0)\<in>R"
-    shows "LIST_FOREACH' (RETURN li) ci fi s0i \<le> \<Down>R (FOREACHci I l c f s0)"
-  proof -
-    from assms(1) have [simp]: "finite l" by (auto simp: list_set_rel_def br_def)
-    show ?thesis
-      unfolding FOREACHc_def FOREACHci_def FOREACHoci_by_LIST_FOREACH
-      apply simp
-      apply (rule LIST_FOREACH_autoref[param_fo, THEN nres_relD])
-      using assms
-      apply auto
-      apply (auto simp: it_to_sorted_list_def nres_rel_def pw_le_iff refine_pw_simps
-        list_set_rel_def br_def)
-      done
-  qed    
-      
-
-  lemma LFOci_refine: (* TODO: Move and generalize! *)
-    assumes "(li,l)\<in>\<langle>A\<rangle>list_set_rel"
-    assumes "\<And>s si. (si,s)\<in>R \<Longrightarrow> ci si \<longleftrightarrow> c s"
-    assumes "\<And>x xi s si. \<lbrakk>(xi,x)\<in>A; (si,s)\<in>R\<rbrakk> \<Longrightarrow> fi xi si \<le> \<Down>R (f x s)"
-    assumes "(s0i,s0)\<in>R"
-    shows "nfoldli li ci fi s0i \<le> \<Down>R (FOREACHci I l c f s0)"
-  proof -
-    from assms LFO_pre_refine[of li l A ci c R fi f s0i s0] show ?thesis
-      unfolding fun_rel_def nres_rel_def LIST_FOREACH'_def
-      apply (simp add: pw_le_iff refine_pw_simps)
-      apply blast+
-      done
-  qed    
-
-  lemma LFOc_refine: (* TODO: Move and generalize! *)
-    assumes "(li,l)\<in>\<langle>A\<rangle>list_set_rel"
-    assumes "\<And>s si. (si,s)\<in>R \<Longrightarrow> ci si \<longleftrightarrow> c s"
-    assumes "\<And>x xi s si. \<lbrakk>(xi,x)\<in>A; (si,s)\<in>R\<rbrakk> \<Longrightarrow> fi xi si \<le> \<Down>R (f x s)"
-    assumes "(s0i,s0)\<in>R"
-    shows "nfoldli li ci fi s0i \<le> \<Down>R (FOREACHc l c f s0)"
-    unfolding FOREACHc_def
-    by (rule LFOci_refine[OF assms])
-
-    
-  lemma LFO_refine: (* TODO: Move and generalize! *)
-    assumes "(li,l)\<in>\<langle>A\<rangle>list_set_rel"
-    assumes "\<And>x xi s si. \<lbrakk>(xi,x)\<in>A; (si,s)\<in>R\<rbrakk> \<Longrightarrow> fi xi si \<le> \<Down>R (f x s)"
-    assumes "(s0i,s0)\<in>R"
-    shows "nfoldli li (\<lambda>_. True) fi s0i \<le> \<Down>R (FOREACH l f s0)"
-    unfolding FOREACH_def
-    apply (rule LFOc_refine)
-    apply (rule assms | simp)+
-    done
-
-  lemma LFOi_refine: (* TODO: Move and generalize! *)
-    assumes "(li,l)\<in>\<langle>A\<rangle>list_set_rel"
-    assumes "\<And>x xi s si. \<lbrakk>(xi,x)\<in>A; (si,s)\<in>R\<rbrakk> \<Longrightarrow> fi xi si \<le> \<Down>R (f x s)"
-    assumes "(s0i,s0)\<in>R"
-    shows "nfoldli li (\<lambda>_. True) fi s0i \<le> \<Down>R (FOREACHi I l f s0)"
-    unfolding FOREACHi_def
-    apply (rule LFOci_refine)
-    apply (rule assms | simp)+
-    done
-
-  (* TODO: Move to refinement framework. Combine with select from CAVA-Base. *)
-  definition "SELECTp P \<equiv> if Ex P then RES {Some x | x. P x} else RETURN None"
-
-  lemma selectp_rule[refine_vcg]: 
-    assumes "\<forall>x. \<not>P x \<Longrightarrow> RETURN None \<le> SPEC \<Phi>"
-    assumes "\<And>x. P x \<Longrightarrow> RETURN (Some x) \<le> SPEC \<Phi>"
-    shows "SELECTp P \<le> SPEC \<Phi>"
-    using assms unfolding SELECTp_def
-    by (auto)
-
-  lemma selectp_refine_eq:
-    "SELECTp P \<le> \<Down>(\<langle>R\<rangle>option_rel) (SELECTp Q) \<longleftrightarrow> 
-    (\<forall>x. P x \<longrightarrow> (\<exists>y. (x,y)\<in>R \<and> Q y)) \<and> ((\<forall>x. \<not>P x) \<longrightarrow> (\<forall>y. \<not>Q y))"
-    by (auto simp: SELECTp_def option_rel_def
-      simp: pw_le_iff refine_pw_simps)
-
-  lemma selectp_refine[refine]:
-    assumes "SPEC P \<le>\<Down>R (SPEC Q)"  
-    assumes "\<And>y. \<forall>x. \<not>P x \<Longrightarrow> \<not>Q y"
-    shows "SELECTp P \<le> \<Down>(\<langle>R\<rangle>option_rel) (SELECTp Q)"
-    unfolding selectp_refine_eq
-    using assms by (auto simp: pw_le_iff refine_pw_simps)
-
-  lemma selectp_refine_Id[refine]:  
-    assumes "\<And>x. P x \<Longrightarrow> Q x"
-    assumes "\<And>y. \<forall>x. \<not>P x \<Longrightarrow> \<not>Q y"
-    shows "SELECTp P \<le> \<Down>Id (SELECTp Q)"
-    using selectp_refine[where R=Id, of P Q] assms by auto
-    
-  lemma selectp_pw[refine_pw_simps]:
-    "nofail (SELECTp P)"  
-    "inres (SELECTp P) r \<longleftrightarrow> (r=None \<longrightarrow> (\<forall>x. \<not>P x)) \<and> (\<forall>x. r=Some x \<longrightarrow> P x)"
-    unfolding SELECTp_def
-    by auto
-
-  lemma selectp_pw_simps[simp]:
-    "nofail (SELECTp P)"
-    "inres (SELECTp P) None \<longleftrightarrow> (\<forall>x. \<not>P x)"
-    "inres (SELECTp P) (Some x) \<longleftrightarrow> P x"
-    by (auto simp: refine_pw_simps)
-
-  context Refine_Monadic_Syntax begin 
-    notation SELECTp (binder "selectp " 10)
-
-    term "selectp x. P x"
-  end
-
-
-definition setsum_impl :: "('a \<Rightarrow> 'b::comm_monoid_add nres) \<Rightarrow> 'a set \<Rightarrow> 'b nres" where
-  "setsum_impl g S \<equiv> foreach S (\<lambda>x a. do { b \<leftarrow> g x; return (a+b)}) 0"
-
-lemma setsum_imp_correct: 
-  assumes [simp]: "finite S"
-  assumes [THEN order_trans, refine_vcg]: "\<And>x. x\<in>S \<Longrightarrow> gi x \<le> (spec r. r=g x)"
-  shows "setsum_impl gi S \<le> (spec r. r=sum g S)"
-  unfolding setsum_impl_def
-  apply (refine_vcg FOREACH_rule[where I="\<lambda>it a. a = sum g (S - it)"])
-  apply (auto simp: it_step_insert_iff algebra_simps)
-  done
-
-
-  lemma int_of_integer_less_iff: "int_of_integer x < int_of_integer y \<longleftrightarrow> x<y"
-    by (simp add: less_integer_def)
-
-  lemma nat_of_integer_less_iff: "x\<ge>0 \<Longrightarrow> y\<ge>0 \<Longrightarrow> nat_of_integer x < nat_of_integer y \<longleftrightarrow> x<y"
-    unfolding nat_of_integer.rep_eq
-    by (auto simp: int_of_integer_less_iff nat_less_eq_zless int_of_integer_less_iff[of 0, simplified])
-    
-      
-(* TODO: Move *)  
-  
+  (* TODO: Move *)  
 lemma uminus_hnr[sepref_import_param]: "(uminus,uminus)\<in>int_rel \<rightarrow> int_rel" by auto  
   
   (* TODO: Move *)  
